Dijkstra/Control/Monad/Rel.lean
@@ -20,8 +20,8 @@ Thus, as an endo-functor, `r` is identified with a characteristic map `r : {α :
 In order for the resulting subfunctor to inherit the structure of a monad, it has to satisfy the following properties:
 
 ```lean
-MonadRel.rel_pure {α : Type u} : ∀ (a : α), r (pure a) (pure a)
-MonadRel.rel_bind {α β : Type u} {x : m α} {y : n α} {f : α → m β} {g : α → n β} : r x y → (∀ a, r (f a) (g a)) → r (x >>= f) (y >>= g)
+MonadRel.pure {α : Type u} : ∀ (a : α), r (pure a) (pure a)
+MonadRel.bind {α β : Type u} {x : m α} {y : n α} {f : α → m β} {g : α → n β} : r x y → (∀ a, r (f a) (g a)) → r (x >>= f) (y >>= g)
 ```
 
 We call such a relation a ***monadic relation***.
@@ -29,11 +29,14 @@ We call such a relation a ***monadic relation***.
 
 universe u v v₁ v₂ v₃ w w₁ w₂
 
-class MonadRel (m : Type u → Type v) [Monad m] (n : Type u → Type w) [Monad n] where
+structure MonadRel (m : Type u → Type v) [Monad m] (n : Type u → Type w) [Monad n] where
   rel {α : Type u} : m α → n α → Prop
-  rel_pure {α : Type u} (a : α) : rel (pure a) (pure a)
-  rel_bind {α β : Type u} {x : m α} {y : n α} {f : α → m β} {g : α → n β} : rel x y → (∀ a, rel (f a) (g a)) → rel (x >>= f) (y >>=g)
+  pure {α : Type u} (a : α) : rel (pure a) (pure a)
+  bind {α β : Type u} {x : m α} {y : n α} {f : α → m β} {g : α → n β} : rel x y → (∀ a, rel (f a) (g a)) → rel (x >>= f) (y >>=g)
 
+/-- This coercion enables one to use `MonadRel` as if it is an ordinary relation. Indeed, if `r : MonadRel m n`, then for `x : m α` and `y : n α`, one can write `r x y` instead of `r.rel x y`.-/
+instance coeMonadRel (m : Type u → Type v) [Monad m] (n : Type u → Type w) [Monad n] : CoeFun (MonadRel m n) (λ _ => {α : Type u} → m α → n α → Prop) where
+  coe r {_} := r.rel
 
 namespace MonadRel
 
@@ -41,36 +44,36 @@ namespace MonadRel
 protected
 def Eq {m : Type u → Type v} [Monad m] : MonadRel m m where
   rel := Eq
-  rel_pure _ := rfl
-  rel_bind h hfg := h ▸ bind_congr hfg
+  pure _ := rfl
+  bind h hfg := h ▸ bind_congr hfg
 
 /-- Invert the direction of a given relation. -/
 def swap {m : Type u → Type v} [Monad m] {n : Type u → Type w} [Monad n] (r : MonadRel m n) : MonadRel n m where
   rel y x := r.rel x y
-  rel_pure a := r.rel_pure a
-  rel_bind hxy hfg := r.rel_bind hxy hfg
+  pure a := r.pure a
+  bind hxy hfg := r.bind hxy hfg
 
 /-- @warning the composition of monadic relations requires `Classical.Choice`. -/
 def comp {m₁ : Type u → Type v₁} [Monad m₁] {m₂ : Type u → Type v₂} [Monad m₂] {m₃ : Type u → Type v₃} [Monad m₃] (r₁ : MonadRel m₁ m₂) (r₂ : MonadRel m₂ m₃) : MonadRel m₁ m₃ where
   rel x z := ∃ y, r₁.rel x y ∧ r₂.rel y z
-  rel_pure a := Exists.intro (Pure.pure a) ⟨r₁.rel_pure a, r₂.rel_pure a⟩
-  rel_bind := by
+  pure a := Exists.intro (Pure.pure a) ⟨r₁.pure a, r₂.pure a⟩
+  bind := by
     dsimp; intro α β x z f h hxz hfh
     cases hxz with | intro y hy =>
     cases Classical.axiomOfChoice hfh with | intro g hg =>
     exists y >>= g
-    exact ⟨r₁.rel_bind hy.left (λ a => (hg a).left), r₂.rel_bind hy.right (λ a => (hg a).right)⟩
+    exact ⟨r₁.bind hy.left (λ a => (hg a).left), r₂.bind hy.right (λ a => (hg a).right)⟩
 
 /-- Pullback of a relation with respect to the left variable. -/
 def pullLeft {m₁ : Type u → Type v₁} [Monad m₁] {m₂ : Type u → Type v₂} [Monad m₂] {n : Type u → Type w} [Monad n] (F : MonadHom m₁ m₂) (r : MonadRel m₂ n) : MonadRel m₁ n where
   rel x y := r.rel (F.app x) y
-  rel_pure a := by dsimp; rw [F.app_pure a]; exact r.rel_pure a
-  rel_bind hxy hfg := by dsimp; rw [F.app_bind]; exact r.rel_bind hxy hfg
+  pure a := by dsimp; rw [F.app_pure a]; exact r.pure a
+  bind hxy hfg := by dsimp; rw [F.app_bind]; exact r.bind hxy hfg
 
 /-- pullback of a relation with respect to the right variable. -/
 def pullRight {m : Type u → Type v} [Monad m] {n₁ : Type u → Type w₁} [Monad n₁] {n₂ : Type u → Type w₂} [Monad n₂] (F : MonadHom n₁ n₂) (r : MonadRel m n₂) : MonadRel m n₁ where
   rel x y := r.rel x (F.app y)
-  rel_pure a := by dsimp; rw [F.app_pure a]; exact r.rel_pure a
-  rel_bind hxy hfg := by dsimp; rw [F.app_bind]; exact r.rel_bind hxy hfg
+  pure a := by dsimp; rw [F.app_pure a]; exact r.pure a
+  bind hxy hfg := by dsimp; rw [F.app_bind]; exact r.bind hxy hfg
 
 end MonadRel
